examples/dm4free/Relational.UnionFind.Forest.fst
@@ -9,57 +9,9 @@ open FStar.DM4F.Heap.ST
 
 type subtree_t = ordset nat (fun x y -> x <= y)
 
-(***** some boring set lemmas *****)
-assume val minus: subtree_t -> subtree_t -> Tot subtree_t
-assume val strict_subset: subtree_t -> subtree_t -> Tot bool
-assume val set_n (n:nat): subtree_t
-
-let lemma_strict_subset_size (s1:subtree_t) (s2:subtree_t)
-  :Lemma (requires (strict_subset s1 s2))
-         (ensures  (subset s1 s2 /\ size s1 < size s2))
-   [SMTPat (strict_subset s1 s2)]
-  = admit ()
-
-let lemma_minus_mem (s1:subtree_t) (s2:subtree_t) (x:nat)
-  :Lemma (requires True) (ensures (mem x (minus s1 s2) = (mem x s1 && not (mem x s2))))
-   [SMTPat (mem x (minus s1 s2))]
-  = admit ()
-
-let lemma_strict_subset_minus_size (s:subtree_t) (s1:subtree_t) (s2:subtree_t)
-  :Lemma (requires (strict_subset s1 s2 /\ subset s1 s /\ subset s2 s))
-         (ensures  (size (minus s s2) < size (minus s s1)))
-   [SMTPat (strict_subset s1 s2); SMTPat (subset s1 s); SMTPat (subset s2 s)]
-  = admit ()
-
-let lemma_disjoint_union_subset (s1:subtree_t) (s2:subtree_t)
-  :Lemma (requires (~ (s1 == empty) /\ ~ (s2 == empty) /\ intersect s1 s2 == empty))
-         (ensures  (strict_subset s1 (union s1 s2) /\ strict_subset s2 (union s1 s2)))
-   [SMTPatOr [[SMTPat (strict_subset s1 (union s1 s2))]; [SMTPat (strict_subset s2 (union s1 s2))]]]
-  = admit ()
-
-let lemma_subset_union (s1:subtree_t) (s2:subtree_t) (n:nat)
-  :Lemma (requires (subset s1 (set_n n) /\ subset s2 (set_n n)))
-         (ensures  (subset (union s1 s2) (set_n n)))
-   [SMTPat (subset (union s1 s2) (set_n n))]
-  = ()
-
-let lemma_strict_subset_transitive (s1:subtree_t) (s2:subtree_t) (s3:subtree_t)
-  :Lemma (requires (strict_subset s1 s2 /\ strict_subset s2 s3))
-         (ensures  (strict_subset s1 s3))
-   [SMTPat (strict_subset s1 s2); SMTPat (strict_subset s2 s3)]
-  = admit ()
-
-let lemma_intersect_transitive (s1:subtree_t) (s2:subtree_t)
-  :Lemma (requires True) (ensures (intersect s1 s2 == intersect s2 s1))
-   [SMTPatOr [[SMTPat (intersect s1 s2)]; [SMTPat (intersect s2 s1)]]]
-  = admit ()
-
-let lemma_intersect_union_empty (s1:subtree_t) (s2:subtree_t) (s3:subtree_t)
-  :Lemma (requires (intersect s1 s3 == empty /\ intersect s2 s3 == empty))
-         (ensures  (intersect (union s1 s2) s3 == empty))
-   [SMTPat (intersect (union s1 s2) s3)]
-  = admit ()
-(***** end boring set lemmas *****)
+let rec set_n (n:nat) :subtree_t =
+  if n = 0 then empty
+  else union (singleton n) (set_n (n - 1))
 
 type id (n:nat) = i:nat{i < n}
 
